Lean4Lean/Experimental/ShapeLogRel.lean
@@ -101,36 +101,11 @@ abbrev ShapeFun (n) := List (Shape n × Shape n)
   | 0 => Shape0.sort
   | _+1 => ShapeS.sort
 
--- def Shape.rank : Shape → Nat
---   | .bot => 0
---   | .sort k => k + 1
---   | .forallE s₁ s₂ =>
---     s₂.attach.foldl (fun n ⟨(a, b), _⟩ => max n (max a.rank b.rank)) s₁.rank + 1
--- decreasing_by all_goals
---   simp; first | omega | have := List.sizeOf_lt_of_mem ‹_›; simp at this; omega
-
--- omit [Params] in
--- theorem Shape.rank_forall_le : (forallE s f).rank ≤ n ↔
---   s.rank < n ∧ ∀ x y, (x, y) ∈ f → x.rank < n ∧ y.rank < n := by
---   simp [rank, Nat.succ_le_iff]; generalize s.rank = i
---   rw [(by simp : (∀ _, _) ↔ (∀ x ∈ f.attach, x.1.1.rank < n ∧ x.1.2.rank < n))]
---   induction f.attach generalizing i <;> simp [*, and_assoc, Nat.max_lt]
-
--- omit [Params] in
--- @[simp] theorem Shape.lt_rank_forall_fst : s.rank < (forallE s f).rank := by
---   simp [← Nat.not_le, rank_forall_le]
-
--- omit [Params] in
--- theorem Shape.lt_rank_forall_snd :
---     (x, y) ∈ f → x.rank < (forallE s f).rank ∧ y.rank < (forallE s f).rank :=
---   rank_forall_le.1 (Nat.le_refl _) |>.2 _ _
-
 def ShapeFun.Compat (R : α → β → Bool) (f : List (α × α)) (f' : List (β × β)) : Bool :=
   f.all fun (x, y) => f'.all fun (x', y') => R x x' → R y y'
 
 def Shape.Compat : ∀ {n}, Shape n → Shape n → Bool
-  | 0, _, _ => true
-  | _+1, .sort, .sort => true
+  | 0, _, _ | _+1, .bot, _ | _+1, _, .bot | _+1, .sort, .sort => true
   | _+1, .forallE s f, .forallE s' f' => s.Compat s' && ShapeFun.Compat Compat f f'
   | _+1, .lam f, .lam f' => ShapeFun.Compat Compat f f'
   | _, _, _ => false
@@ -152,6 +127,8 @@ instance : DecidableRel (α := Shape n) (· ≤ ·) := fun x y => inferInstanceA
 
 omit [Params] in
 @[simp] theorem Shape.bot_le : Shape.bot ≤ (s : Shape n) := by cases n <;> rfl
+
+def ShapeFun.bot : ShapeFun n := [(.bot, .bot)]
 
 omit [Params] in
 theorem ShapeFun.LE.def {f f' : ShapeFun n} : ShapeFun.LE f f' ↔
@@ -233,6 +210,11 @@ theorem Shape.lift_lift {s : Shape n₁} (le : n₁ ≤ n₂ ∨ n₃ ≤ n₂) 
       -- case sort i h1 => split <;> split <;> simp [lift, *]; grind
 
 omit [Params] in
+theorem ShapeFun.lift_lift {s : ShapeFun n₁} (le : n₁ ≤ n₂ ∨ n₃ ≤ n₂) :
+    (lift Shape.lift (lift Shape.lift s : ShapeFun n₂) : ShapeFun n₃) =
+    lift Shape.lift s := by simp [ShapeFun.lift, Shape.lift_lift le]
+
+omit [Params] in
 theorem Shape.lift_le_lift {s t : Shape n} (le : n ≤ m) : (s.lift : Shape m) ≤ t.lift ↔ s ≤ t := by
   dsimp [(· ≤ ·), Shape.LE]; rw [← Bool.eq_iff_iff]
   induction n generalizing m with
@@ -248,6 +230,10 @@ theorem Shape.lift_le_lift {s t : Shape n} (le : n ≤ m) : (s.lift : Shape m) �
     -- have sif {i} (h : i ≤ n) : (if h : i ≤ m then .sort i h else .bot : Shape (m+1)) =
     --     .sort i (Nat.le_trans h le) := dif_pos _
     cases s <;> cases t <;> simp [ble, lift, *]
+
+omit [Params] in
+theorem Shape.lift_le_bot {s : Shape n} (h : n ≤ m) : s.lift (m := m) ≤ .bot ↔ s = .bot := by
+  rw [← le_bot, ← lift_bot, Shape.lift_le_lift h]
 
 omit [Params] in
 theorem Shape.lift_mono {s t : Shape n} : s ≤ t → (s.lift : Shape m) ≤ t.lift := by
@@ -270,6 +256,13 @@ theorem Shape.lift_mono {s t : Shape n} : s ≤ t → (s.lift : Shape m) ≤ t.l
       -- · split <;> split <;> simp [ble]; omega
       · grind
       · grind
+
+omit [Params] in
+theorem ShapeFun.lift_mono {s t : ShapeFun n} : s.LE t →
+    LE (lift Shape.lift s : ShapeFun m) (lift Shape.lift t) := by
+  simp only [ShapeFun.LE, ShapeFun.ble, List.all_eq_true, List.any_eq_true, Bool.and_eq_true,
+    ShapeFun.lift, List.any_map, List.all_map, Function.comp_apply]
+  exact fun H _ h1 => let ⟨_, h2, h3, h4⟩ := H _ h1; ⟨_, h2, Shape.lift_mono h3, Shape.lift_mono h4⟩
 
 -- def ShapeFun.plift (lift : α → β × Option β) (x : List (α × α)) :
 --     List (β × β) × Option (List (β × β)) :=
@@ -335,23 +328,69 @@ theorem Shape.LE.trans {s t u : Shape n} : s ≤ t → t ≤ u → s ≤ u := by
     cases s <;> cases t <;> simp [ble] <;> cases u <;> simp [ble] <;>
       [exact fun h1 h2 h3 h4 => ⟨ih h1 h3, ihf h2 h4⟩; exact ihf]
 
+omit [Params] in
+theorem ShapeFun.LE.trans {s t u : ShapeFun n} : s.LE t → t.LE u → s.LE u := by
+  simp only [ShapeFun.LE, ShapeFun.ble, List.all_eq_true, List.any_eq_true, Bool.and_eq_true]
+  rintro h1 h2 x hx; let ⟨_, hy, x1, x2⟩ := h1 _ hx; let ⟨_, hz, y1, y2⟩ := h2 _ hy
+  exact ⟨_, hz, Shape.LE.trans y1 x1, Shape.LE.trans x2 y2⟩
+
 def Shape.Join (x y z : Shape n) := ∀ w, z ≤ w ↔ x ≤ w ∧ y ≤ w
+def ShapeFun.Join (x y z : ShapeFun n) := ∀ w, z.LE w ↔ x.LE w ∧ y.LE w
+
+theorem Shape.Compat.lift {x y : Shape n} (le : n ≤ m) :
+    (x.lift : Shape m).Compat y.lift ↔ x.Compat y := sorry
+
+theorem ShapeFun.Compat.lift {x y : ShapeFun n} (le : n ≤ m) :
+    Compat Shape.Compat (lift Shape.lift x : ShapeFun m) (lift Shape.lift y) ↔
+    Compat Shape.Compat x y := sorry
+
+omit [Params] in
+theorem Shape.Join.le (H : Join x y z) : x ≤ z ∧ y ≤ z := (H _).1 .rfl
+
+omit [Params] in
+theorem Shape.join_self : Join x x y ↔ x ≤ y ∧ y ≤ x :=
+  ⟨fun H => ⟨((H _).1 .rfl).1, (H _).2 ⟨.rfl, .rfl⟩⟩,
+   fun ⟨H1, H2⟩ _ => ⟨fun h => ⟨H1.trans h, H1.trans h⟩, fun h => H2.trans h.1⟩⟩
+
+theorem Shape.Compat.def {x y : Shape n} : x.Compat y ↔ ∃ z, x ≤ z ∧ y ≤ z := sorry
+
+theorem Shape.Join.compat (H : Join x y z) : x.Compat y := Compat.def.2 ⟨_, (H _).1 .rfl⟩
+
+theorem Shape.Join.forallE (H : Join x y z) : x.Compat y := sorry
+
+theorem Shape.Join.lift {x y : Shape n} (le : n ≤ m) :
+    (x.lift : Shape m).Join y.lift z.lift ↔ x.Join y z := sorry
 
 def ShapeFun.join (join : Shape n → Shape n → Shape n)
     (f f' : List (Shape n × Shape n)) : List (Shape n × Shape n) := by
-  refine f.attach.foldl (init := []) fun l ⟨(x, y), hxy⟩ => ?_
-  refine f'.attach.foldl (init := l) fun l ⟨(x', y'), hxy'⟩ => ?_
+  refine f.foldl (init := []) fun l (x, y) => ?_
+  refine f'.foldl (init := l) fun l (x', y') => ?_
   refine if x.Compat x' then ?_ else l
   let jx := join x x'
   let jy := join y y'
   exact l.map fun (z, w) => (z, if z ≤ jx then join w jy else w)
 
 def Shape.join : ∀ {n}, Shape n → Shape n → Shape n
-  | 0, s, _ | _+1, .bot, s | _+1, s, .bot => s
-  | _+1, .sort, .sort => .sort
+  | 0, s, .bot | 0, .bot, s | _+1, .bot, s | _+1, s, .bot => s
+  | 0, .sort, .sort | _+1, .sort, .sort => .sort
   | _+1, .forallE s f, .forallE s' f' => .forallE (join s s') (ShapeFun.join join f f')
   | _+1, .lam f, .lam f' => .lam (ShapeFun.join join f f')
   | _+1, _, _ => .bot
+
+theorem Shape.Join.mk (H : x.Compat y) : Join x y (x.join y) := sorry
+
+theorem ShapeFun.Join.mk (H : Compat Shape.Compat x y) : Join x y (join Shape.join x y) := sorry
+
+theorem Shape.Join.iff : Join x y z ↔ x.Compat y ∧ x.join y ≤ z ∧ z ≤ x.join y :=
+  ⟨fun h => ⟨h.compat, (mk h.compat _).2 h.le, (h _).2 (mk h.compat).le⟩,
+   fun ⟨h1, h2, h3⟩ _ => .trans ⟨(.trans h2 ·), (.trans h3 ·)⟩ (mk h1 _)⟩
+
+theorem Shape.lift_join {x y : Shape n} (le : n ≤ m) :
+    ((x.join y).lift : Shape m) = x.lift.join y.lift := sorry
+
+theorem ShapeFun.lift_join {x y : ShapeFun n} (le : n ≤ m) :
+    (lift Shape.lift (ShapeFun.join Shape.join x y) : ShapeFun m) =
+    join Shape.join (lift Shape.lift x) (lift Shape.lift y) := sorry
 
 def ShapeFun.maxBelow (s : ShapeFun n) : Shape n × Shape n :=
   (s.find? fun (x, _) => s.all fun (x', _) => x' ≤ x).getD (.bot, .bot)
@@ -359,16 +398,57 @@ def ShapeFun.maxBelow (s : ShapeFun n) : Shape n × Shape n :=
 def ShapeFun.app (s : ShapeFun n) (a : Shape n) : Shape n :=
   maxBelow (s.filter (·.1 ≤ a)) |>.2
 
+omit [Params] in
+theorem ShapeFun.app_of_mem {f : ShapeFun n} (h : (x, y) ∈ f) : f.app x = y :=
+  sorry
+
+omit [Params] in
+theorem ShapeFun.uniq {f : ShapeFun n} (h1 : (x, y) ∈ f) (h2 : (x', y') ∈ f)
+    (h3 : x ≤ x') (h4 : y' ≤ y) : x = x' ∧ y = y' :=
+  sorry
+
+omit [Params] in
+theorem ShapeFun.app_eq (f : ShapeFun n) (x) : ∃ x' y', x' ≤ x ∧ (x', y') ∈ f ∧ f.app x = y' :=
+  sorry
+
+omit [Params] in
 theorem ShapeFun.app_mono_l {f f' : ShapeFun n} : f.LE f' → ∀ a, f.app a ≤ f'.app a :=
   sorry
 
+omit [Params] in
 theorem ShapeFun.app_mono_r {f : ShapeFun n} : a ≤ a' → f.app a ≤ f.app a' :=
+  sorry
+
+omit [Params] in
+theorem ShapeFun.uniq_l {f : ShapeFun n} (h1 : (x, y) ∈ f) (h2 : (x', y') ∈ f)
+    (h3 : x ≤ x') (h4 : x' ≤ x) : x = x' ∧ y = y' :=
+  ShapeFun.uniq h1 h2 h3 (app_of_mem h1 ▸ app_of_mem h2 ▸ app_mono_r h4)
+
+@[simp] theorem ShapeFun.bot_app : (@ShapeFun.bot n).app x = .bot := sorry
+
+omit [Params] in
+@[simp] theorem ShapeFun.lift_app :
+    ((app f a : Shape n).lift : Shape m) = app (lift Shape.lift f) a.lift  := by
   sorry
 
 def Shape.app : Shape (n + 1) → Shape n → Shape n
   | .lam f, x => ShapeFun.app f x
   | _, _ => .bot
 
+@[simp] theorem Shape.bot_app : (@Shape.bot (n+1)).app x = .bot := rfl
+
+omit [Params] in
+@[simp] theorem Shape.lift_app :
+    ((app f a : Shape n).lift : Shape m) = app f.lift a.lift  := by
+  sorry
+
+def ShapeFun.single (x y : Shape n) : ShapeFun n :=
+  (x, y) :: if x ≤ .bot then [] else [(.bot, .bot)]
+
+theorem ShapeFun.single_app : (ShapeFun.single x y).app x' = if x ≤ x' then y else .bot := by
+  sorry
+
+omit [Params] in
 theorem Shape.app_mono_l {f f' : Shape (n + 1)} (le : f ≤ f') (a) : f.app a ≤ f'.app a := by
   unfold app; split <;> [split; simp]
   · exact ShapeFun.app_mono_l le _
@@ -376,34 +456,78 @@ theorem Shape.app_mono_l {f f' : Shape (n + 1)} (le : f ≤ f') (a) : f.app a �
 
 def Shape.hasType : ∀ {n}, Shape n → Shape n → Bool
   | _+1, .bot, .forallE a b | _+1, .forallE a b, .sort =>
-    a.hasType .sort && b.all fun (x, y) => x.hasType a && y.hasType .sort
+    b.all fun (x, y) => x.hasType a && y.hasType .sort
   | 0, .bot, _ | _+1, .bot, .bot | _+1, .bot, .sort
   | 0, .sort, .sort | _+1, .sort, .sort => true
   | _+1, .lam f, .forallE a b =>
-    a.hasType .sort && b.all (fun (x, y) => x.hasType a && y.hasType .sort) &&
+    b.all (fun (x, y) => x.hasType a && y.hasType .sort) &&
     f.all (fun (x, y) => x.hasType a && y.hasType (ShapeFun.app b x))
   | _, _, _ => false
 
 def Shape.HasType : Shape n → Shape n → Prop := (hasType · ·)
 
+def Shape.HasDom (f : ShapeFun n) (a : Shape n) :=
+  ∀ x, ∃ x', x' ≤ x ∧ HasType x' a ∧ f.app x ≤ f.app x'
+
+omit [Params] in
+theorem Shape.HasDom.def : HasDom f a ↔ ∀ x y, (x, y) ∈ f → x.HasType a := by
+  refine ⟨fun H x y h => ?_, fun H x => ?_⟩
+  · sorry
+  · sorry
+
+omit [Params] in
+theorem Shape.HasDom.lift (le : n ≤ m) :
+    HasDom (n := m) (.lift Shape.lift f) a.lift ↔ HasDom f a := by
+  sorry
+
+def Shape.HasTypePi (b : ShapeFun n) (a : Shape n) :=
+  Shape.HasDom b a ∧ ∀ x, HasType x a → HasType (b.app x) .sort
+
+omit [Params] in
+theorem Shape.HasTypePi.def {b : ShapeFun n} :
+    HasTypePi b a ↔ Shape.HasDom b a ∧ ∀ x y, (x, y) ∈ b → y.HasType .sort := by
+  refine and_congr_right fun H1 => ⟨fun H x y h => ?_, fun H x h => ?_⟩
+  · exact b.app_of_mem h ▸ H _ (Shape.HasDom.def.1 H1 _ _ h)
+  · have ⟨_, _, h1, h2, h3⟩ := b.app_eq x
+    exact h3 ▸ H _ _ h2
+
+def Shape.HasTypeLam (f : ShapeFun n) (a : Shape n) (b : ShapeFun n) :=
+  Shape.HasTypePi b a ∧ Shape.HasDom f a ∧
+  ∀ x, HasType x a → HasType (f.app x) (b.app x)
+
+omit [Params] in
+theorem Shape.HasType.mono_r {m a a' : Shape n} (ha : a ≤ a') :
+    HasType a' .sort → HasType m a → HasType m a' := sorry
+
+omit [Params] in
+theorem Shape.HasTypeLam.def {b : ShapeFun n} : HasTypeLam f a b ↔
+    Shape.HasTypePi b a ∧ Shape.HasDom f a ∧ ∀ x y, (x, y) ∈ f → y.HasType (b.app x) := by
+  refine and_congr_right fun H1 => and_congr_right fun H2 => ⟨fun H x y h => ?_, fun H x h => ?_⟩
+  · exact f.app_of_mem h ▸ H _ (Shape.HasDom.def.1 H2 _ _ h)
+  · have ⟨_, _, h1, h2, h3⟩ := f.app_eq x
+    exact .mono_r (ShapeFun.app_mono_r h1) (H1.2 _ h) (h3 ▸ H _ _ h2)
+
 inductive Shape.HasTypeU : ∀ {n}, Shape n → Shape n → Prop
   | bot : HasType x .sort → HasTypeU .bot x
   | sort : HasTypeU .sort .sort
-  | forallE : HasType (n := n) a .sort →
-    (∀ x y, (x, y) ∈ b → HasType x a ∧ HasType y .sort) →
-    HasTypeU (n := n+1) (.forallE a b) .sort
-  | lam : HasType (n := n) a .sort →
-    (∀ x y, (x, y) ∈ b → HasType x a ∧ HasType y .sort) →
-    (∀ x y, (x, y) ∈ (f : ShapeFun n) → HasType x a ∧ HasType y (ShapeFun.app b x)) →
-    HasTypeU (n := n+1) (.lam f) (.forallE a b)
+  | forallE : HasTypePi (n := n) b a → HasTypeU (n := n+1) (.forallE a b) .sort
+  | lam : HasTypeLam (n := n) f a b → HasTypeU (n := n+1) (.lam f) (.forallE a b)
 
 omit [Params] in
 theorem Shape.HasType.unfold {m a : Shape n} : HasType m a → HasTypeU m a := by
   unfold HasType hasType; split <;> simp <;> intros <;> constructor <;> try grind [HasType]
   · simp [HasType, hasType]; grind
+  · rename_i a b H
+    refine ⟨HasDom.def.2 fun _ _ h => (H _ _ h).1, fun x h => ?_⟩
+    have ⟨_, _, h1, h2, h3⟩ := ShapeFun.app_eq b x
+    exact h3 ▸ (H _ _ h2).2
   · rename_i x; cases x <;> rfl
   · rfl
   · rfl
+  · rename_i h1 h2
+    exact Shape.HasTypeLam.def.2 ⟨Shape.HasTypePi.def.2 ⟨
+      Shape.HasDom.def.2 fun _ _ h => (h1 _ _ h).1, fun _ _ h => (h1 _ _ h).2⟩,
+      Shape.HasDom.def.2 fun _ _ h => (h2 _ _ h).1, fun _ _ h => (h2 _ _ h).2⟩
 
 omit [Params] in
 theorem Shape.HasType.unfold_iff {m a : Shape n} : HasType m a ↔ HasTypeU m a := by
@@ -413,19 +537,55 @@ theorem Shape.HasType.unfold_iff {m a : Shape n} : HasType m a ↔ HasTypeU m a 
   | bot h =>
     cases h.unfold with
     | bot | sort => cases n <;> rfl
-    | forallE => simp; grind [HasType]
+    | forallE => simpa [HasType, hasType] using h
   | sort => cases n <;> rfl
-  | _ => simp <;> grind [HasType]
+  | forallE h =>
+    have := HasTypePi.def.1 h
+    have := HasDom.def.1 this.1
+    simp; grind [HasType]
+  | lam h =>
+    have ⟨h1, h2, _⟩ := HasTypeLam.def.1 h
+    have := HasDom.def.1 h2
+    have := HasTypePi.def.1 h1
+    have := HasDom.def.1 this.1
+    simp; grind [HasType]
+
+omit [Params] in
+theorem Shape.HasType.bot : HasType (n := n) x .sort → HasType .bot x := (unfold_iff.2 <| .bot ·)
+omit [Params] in
+theorem Shape.HasType.sort : HasType (n := n) .sort .sort := unfold_iff.2 .sort
+omit [Params] in
+theorem Shape.HasType.forallE : HasTypePi (n := n) b a →
+    HasType (n := n+1) (.forallE a b) .sort := (unfold_iff.2 <| .forallE ·)
+omit [Params] in
+theorem Shape.HasType.lam : HasTypeLam (n := n) f a b →
+    HasType (n := n+1) (.lam f) (.forallE a b) := (unfold_iff.2 <| .lam ·)
+
+omit [Params] in
+theorem Shape.HasType.bot_r (H : HasType (n := n) x .bot) : x = .bot := by
+  cases n <;> cases H.unfold <;> rfl
 
 omit [Params] in
 theorem Shape.HasType.isType {m a : Shape n} (h : HasType m a) : HasType a .sort := by
   cases h.unfold with
   | bot h1 => exact h1
-  | sort | forallE => exact unfold_iff.2 .sort
-  | lam h1 h2 => exact unfold_iff.2 <| .forallE h1 h2
+  | sort | forallE => exact .sort
+  | lam h1 => exact .forallE h1.1
 
-theorem Shape.HasType.mono_r {m a a' : Shape n} (ha : a ≤ a') :
-    HasType a' .sort → HasType m a → HasType m a' := sorry
+theorem Shape.HasDom.isType (H : Shape.HasDom f a) : a.HasType .sort :=
+  let ⟨_, _, h, _⟩ := H .bot; h.isType
+
+theorem Shape.HasType.lift (h : n ≤ n') :
+    HasType (n := n') m.lift a.lift ↔ HasType (n := n) m a := sorry
+
+omit [Params] in
+theorem Shape.HasType.join (hJ : Join m₁ m₂ m) :
+    HasType m₁ a → HasType m₂ a → HasType m a := sorry
+
+omit [Params] in
+theorem Shape.HasType.mono_l {m a : Shape n}
+    (hm1 : m ≤ m') (hm2 : m' ≤ m) (H : HasType m a) : HasType m' a :=
+  .join (Shape.join_self.2 ⟨hm1, hm2⟩) H H
 
 theorem Shape.HasType.lam_app
     (H : ∀ x y, (x, y) ∈ (f : ShapeFun n) → HasType x a ∧ HasType y (ShapeFun.app b x))
@@ -440,94 +600,540 @@ theorem Shape.HasType.maximal
     (ha : a ≤ a') (ht : HasType x' a') :
     ∃ x, HasType x a ∧ x ≤ x' ∧ ShapeFun.app f x = ShapeFun.app f x' := sorry
 
+omit [Params] in
+theorem Shape.HasDom.single : HasDom (ShapeFun.single x y) a ↔ x.HasType a := by
+  simp [Shape.HasDom.def, ShapeFun.single, or_imp, forall_and]
+  intro h _ _ _ rfl _; exact .bot h.isType
+
+omit [Params] in
+theorem Shape.HasDom.mono (le : a ≤ a') (h : a'.HasType .sort) (H : HasDom f a) : HasDom f a' :=
+  fun x => let ⟨_, h1, h2, h3⟩ := H x; ⟨_, h1, .mono_r le h h2, h3⟩
+
 def ShapeFun.WF (WF : Shape n → Bool) (f : ShapeFun n) : Bool :=
-  (f.attach.all fun ⟨(x, y), _⟩ => WF x && WF y) && f.any (·.1 ≤ .bot) &&
-  f.all fun (x, y) => f.all fun (x', y') =>
+  (f.all fun (x, y) => WF x && WF y) && f.any (·.1 ≤ .bot) &&
+  (f.all fun (x, y) => f.all fun (x', y') =>
     (x.Compat x' → (y.Compat y' && let j := x.join x'; f.any fun (z, _) => z ≤ j && j ≤ z)) &&
-    (x ≤ x' → y ≤ y')
+    (x ≤ x' → y ≤ y')) &&
+  f.Pairwise fun (x, y) (x', y') => x ≤ x' → ¬y' ≤ y
 
 def Shape.WF : ∀ {n}, Shape n → Bool
   | 0, _ | _+1, .bot | _+1, .sort .. => true
   | _+1, .forallE s f => s.WF && ShapeFun.WF WF f
   | _+1, .lam f => ShapeFun.WF WF f
 
+def Valuation := Nat → Σ n, Shape n
+
+def Valuation.nil : Valuation := fun _ => ⟨0, .bot⟩
+def Valuation.push (ρ : Valuation) (u : Shape n) : Valuation
+  | 0 => ⟨_, u⟩
+  | n+1 => ρ n
+
+def Valuation.LE (ρ ρ' : Valuation) : Prop :=
+  ∀ n m, (ρ n).1 ≤ m → (ρ' n).1 ≤ m → (ρ n).2.lift (m := m) ≤ (ρ' n).2.lift (m := m)
+
+omit [Params] in
+theorem Valuation.LE.rfl {ρ : Valuation} : ρ.LE ρ :=
+  fun _ _ _ _ => .rfl
+
+omit [Params] in
+theorem Valuation.LE.push' {ρ ρ' : Valuation} (le1 : n ≤ m) (le2 : n' ≤ m) :
+    (ρ.push (n := n) a).LE (ρ'.push (n := n') a') ↔ ρ.LE ρ' ∧ a.lift (m := m) ≤ a'.lift := by
+  refine ⟨fun H => ⟨fun _ _ h1 h2 => H (_+1) _ h1 h2, ?_⟩, ?_⟩
+  · exact H 0 _ le1 le2
+  · rintro ⟨H1, H2⟩ (_|n) m' h1 h2
+    · have := Shape.lift_mono (m := max m m') H2
+      apply (Shape.lift_le_lift (Nat.le_max_right m m')).1
+      rw [Shape.lift_lift (.inl le1), Shape.lift_lift (.inl le2)] at this
+      rwa [Shape.lift_lift (.inl h1), Shape.lift_lift (.inl h2)]
+    · exact H1 _ _ h1 h2
+
+omit [Params] in
+theorem Valuation.LE.push {ρ ρ' : Valuation} : (ρ.push a).LE (ρ'.push a') ↔ ρ.LE ρ' ∧ a ≤ a' := by
+  rw [Valuation.LE.push' (Nat.le_refl _) (Nat.le_refl _), Shape.lift_le_lift (Nat.le_refl _)]
+
+inductive LE_Interp : Valuation → ∀ {n}, Shape n → SExpr → Prop
+  | bot : LE_Interp ρ .bot M
+  -- | le : m ≤ m' → LE_Interp ρ m' M → LE_Interp ρ m M
+  -- | lift : n ≤ n' → LE_Interp (n := n) ρ m M → LE_Interp (n := n') ρ m.lift M
+  | bvar : (ρ i).1 ≤ n' → n ≤ n' → m.lift (m := n') ≤ (ρ i).2.lift → LE_Interp (n := n) ρ m (.bvar i)
+  | sort : m ≤ .sort → LE_Interp ρ m (.sort i)
+  | app : LE_Interp ρ f F → LE_Interp ρ a A → m ≤ f.app a → LE_Interp ρ m (.app F A pat)
+  | lam : LE_Interp (n := n) ρ a A →
+    Shape.HasDom f a → (∀ x, x.HasType a → LE_Interp (ρ.push x) ((f : ShapeFun n).app x) F) →
+    m ≤ .lam f → LE_Interp (n := n+1) ρ m (.lam A F)
+  | forallE : LE_Interp (n := n) ρ b B → LE_Interp (n := n) ρ b' B →
+    Shape.HasDom f b' → (∀ x, x.HasType b' → LE_Interp (ρ.push x) ((f : ShapeFun n).app x) F) →
+    m ≤ .forallE b f → LE_Interp (n := n+1) ρ m (.forallE B F)
+
+theorem LE_Interp.mono : m ≤ m' → LE_Interp ρ m' M → LE_Interp ρ m M := sorry
+theorem LE_Interp.mono_l : ρ.LE ρ' → LE_Interp ρ m M → LE_Interp ρ' m M := sorry
+theorem LE_Interp.lift : n ≤ n' → (LE_Interp (n := n') ρ m.lift M ↔ LE_Interp (n := n) ρ m M) := sorry
+theorem LE_Interp.weak (H : LE_Interp ρ m M) : LE_Interp (ρ.push x) m M.lift := sorry
+theorem LE_Interp.weak_iff : LE_Interp (ρ.push x) m M.lift ↔ LE_Interp ρ m M := sorry
+theorem LE_Interp.inst : LE_Interp (n := n) ρ f (F.inst A) ↔
+    ∃ m a, LE_Interp (n := n) (ρ.push a) f F ∧ LE_Interp (n := m) ρ a A := sorry
+theorem LE_Interp.bvar_iff :
+    LE_Interp (n := n) ρ m (.bvar i) ↔
+    ∃ k, n ≤ k ∧ (ρ i).1 ≤ k ∧ m.lift (m := k) ≤ (ρ i).2.lift := sorry
+
+theorem LE_Interp.join (J : m₁.Join m₂ m) (H1 : LE_Interp ρ m₁ M) (H2 : LE_Interp ρ m₂ M) :
+    LE_Interp ρ m M := sorry
+
+theorem LE_Interp.compat (H1 : LE_Interp ρ m₁ M) (H2 : LE_Interp ρ m₂ M) : m₁.Compat m₂ := sorry
+
+theorem LE_Interp.le_sort (H : LE_Interp ρ m (.sort u)) : m ≤ .sort := by
+  generalize eq : SExpr.sort u = M at H
+  induction H with cases eq
+  | bot => exact Shape.bot_le
+  | sort h => exact h
+
+inductive Valuation.Fits : (Γ Δ : List SExpr) → Valuation → Prop
+  | nil : Valuation.Fits Γ Γ .nil
+  | cons : Valuation.Fits Γ Δ ρ →
+    (∀ {n a}, LE_Interp (n := n) ρ a A →
+      ∃ n' a', n ≤ n' ∧ a.lift (m := n') ≤ a' ∧ LE_Interp ρ a' A ∧ a'.HasType .sort) →
+    LE_Interp (n := n) ρ a A → x.HasType a →
+    Valuation.Fits Γ (A::Δ) (ρ.push x)
+
+def InterpTyped (ρ : Valuation) (m : Shape n) (M A : SExpr) :=
+  ∃ n' m' a, n ≤ n' ∧ m.lift (m := n') ≤ m' ∧
+    LE_Interp ρ m' M ∧ LE_Interp ρ a A ∧ m'.HasType a
+
+theorem InterpTyped.mk (h1 : (m : Shape n) ≤ m') (h2 : LE_Interp ρ m' M)
+    (h3 : LE_Interp ρ a A) (h4 : m'.HasType a) : InterpTyped ρ m M A :=
+  ⟨_, _, _, Nat.le_refl _, Shape.lift_self.symm ▸ h1, h2, h3, h4⟩
+
+theorem InterpTyped.bot : InterpTyped (n := n) ρ .bot M A :=
+  .mk .rfl .bot .bot (.bot <| .bot .sort)
+
+theorem LE_Interp.sound_bot :
+    (LE_Interp (n := n) ρ .bot M ↔ LE_Interp (n := n) ρ .bot N) ∧
+    (LE_Interp (n := n) ρ .bot M → InterpTyped (n := n) ρ .bot M A) :=
+  ⟨⟨fun _ => .bot, fun _ => .bot⟩, fun _ => .bot⟩
+
+theorem LE_Interp.sound_app
+    (H1 : ∀ {n} {m : Shape n}, LE_Interp ρ m f → InterpTyped ρ m f (.forallE A B))
+    (H2 : ∀ {n} {m : Shape n}, LE_Interp ρ m (B.inst a) →
+      ∃ n' a', n ≤ n' ∧ m.lift (m := n') ≤ a' ∧ LE_Interp ρ a' (B.inst a) ∧ a'.HasType .sort)
+    {m : Shape n} (h1 : LE_Interp ρ m (f.app a pat)) :
+    InterpTyped ρ m (f.app a pat) (B.inst a) := by
+  by_cases hm : m = .bot; · exact hm ▸ .bot
+  cases h1 with | bot => exact .bot | app h1 h2 h3
+  have ⟨n', f, s, le, a1, a2, a3, a4⟩ := H1 h1
+  have hf : f ≠ .bot := fun h => by
+    subst h; cases (Shape.lift_le_bot le).1 a1; cases hm (Shape.le_bot.1 h3)
+  have hs : s ≠ .bot := fun h => by subst h; cases a4.bot_r; cases hf rfl
+  cases a3 with | bot => cases hs rfl | @forallE _ n' _ _ _ _ _ s b1 b2 b3 b4 b5
+  replace le := Nat.le_of_succ_le_succ le
+  cases s with simp [Shape.LE.def] at b5 | bot => cases hs rfl | forallE
+  cases a4.unfold with | bot => cases hf rfl | lam c1
+  refine
+    have h2 := (LE_Interp.lift le).2 h2
+    have ⟨_, d1, d2, d3⟩ := b3 _
+    have ⟨m', _, le', g1, g2, g3⟩ := H2 (LE_Interp.inst.2 ⟨_, _, b4 _ d2, .mono d1 h2⟩)
+    have ⟨_, e1, e2, e3⟩ := c1.2.1 _
+    have := (c1.2.2 _ e2).mono_l (ShapeFun.app_mono_r e1) e3
+    ⟨_, _, _, Nat.le_trans le le', ?_, (LE_Interp.lift le').2 (.app a2 h2 .rfl),
+      g2, g3.mono_r ?_ ((Shape.HasType.lift le').2 this)⟩
+  · rw [← Shape.lift_lift (.inl le)]
+    exact Shape.lift_mono <| (Shape.lift_app ▸ Shape.lift_mono h3).trans (Shape.app_mono_l a1 _)
+  · refine (Shape.lift_mono ?_).trans g1
+    exact (ShapeFun.app_mono_l b5.2 _).trans <| (ShapeFun.app_mono_r e1).trans d3
+
+theorem LE_Interp.sound_lam
+    (H1 : ∀ {n} {m : Shape n}, LE_Interp ρ m f → InterpTyped ρ m f (.forallE A B))
+    (H2 : ∀ {n} {m : Shape n}, LE_Interp ρ m (B.inst a) →
+      ∃ n' a', n ≤ n' ∧ m.lift (m := n') ≤ a' ∧ LE_Interp ρ a' (B.inst a) ∧ a'.HasType .sort)
+    {m : Shape n} (h1 : LE_Interp ρ m (f.app a pat)) :
+    InterpTyped ρ m (f.app a pat) (B.inst a) := by
+  by_cases hm : m = .bot; · exact hm ▸ .bot
+  cases h1 with | bot => exact .bot | app h1 h2 h3
+  have ⟨n', f, s, le, a1, a2, a3, a4⟩ := H1 h1
+  have hf : f ≠ .bot := fun h => by
+    subst h; cases (Shape.lift_le_bot le).1 a1; cases hm (Shape.le_bot.1 h3)
+  have hs : s ≠ .bot := fun h => by subst h; cases a4.bot_r; cases hf rfl
+  cases a3 with | bot => cases hs rfl | @forallE _ _ _ _ _ _ _ s b1 b2 b3 b4 b5
+  replace le := Nat.le_of_succ_le_succ le
+  cases s with simp [Shape.LE.def] at b5 | bot => cases hs rfl | forallE
+  cases a4.unfold with | bot => cases hf rfl | lam c1
+  refine
+    have h2 := (LE_Interp.lift le).2 h2
+    have ⟨_, d1, d2, d3⟩ := b3 _
+    have ⟨m', _, le', g1, g2, g3⟩ := H2 (LE_Interp.inst.2 ⟨_, _, b4 _ d2, .mono d1 h2⟩)
+    have ⟨_, e1, e2, e3⟩ := c1.2.1 _
+    have := (c1.2.2 _ e2).mono_l (ShapeFun.app_mono_r e1) e3
+    ⟨_, _, _, Nat.le_trans le le', ?_, (LE_Interp.lift le').2 (.app a2 h2 .rfl),
+      g2, g3.mono_r ?_ ((Shape.HasType.lift le').2 this)⟩
+  · rw [← Shape.lift_lift (.inl le)]
+    exact Shape.lift_mono <| (Shape.lift_app ▸ Shape.lift_mono h3).trans (Shape.app_mono_l a1 _)
+  · refine (Shape.lift_mono ?_).trans g1
+    exact (ShapeFun.app_mono_l b5.2 _).trans <| (ShapeFun.app_mono_r e1).trans d3
+
+theorem LE_Interp.sound (H : Γ ⊢ M ≡ N : A)
+    (W : Valuation.Fits Γ₀ Γ ρ) {m : Shape n} :
+    (LE_Interp ρ m M ↔ LE_Interp ρ m N) ∧
+    (LE_Interp ρ m M → InterpTyped ρ m M A) := by
+  have hsort {ρ A U}
+      (H : ∀ {n a}, LE_Interp (n := n) ρ a A → InterpTyped (n := n) ρ a A (.sort U))
+      {n a} (h : LE_Interp (n := n) ρ a A) :
+      ∃ n' a', n ≤ n' ∧ a.lift (m := n') ≤ a' ∧ LE_Interp ρ a' A ∧ a'.HasType .sort := by
+    have ⟨n', a', u', le, h1, h2, h3, h4⟩ := H h; refine ⟨_, _, le, h1, h2, ?_⟩
+    cases h3 with | bot => cases h4.bot_r; exact .bot .sort | sort h3
+    obtain rfl | rfl := Shape.le_sort.1 h3; · cases h4.bot_r; exact .bot .sort
+    exact h4
+  replace H := H.strong
+  induction H generalizing n m ρ with
+  | @bvar _ i A h =>
+    refine ⟨.rfl, fun h => ?_⟩
+    generalize eq : SExpr.bvar i = M at h
+    induction h with cases eq
+    | bot => exact .mk .rfl .bot .bot (.bot <| .bot .sort)
+    | bvar a1 a2 a3
+    induction W generalizing i A with
+    | nil => cases (Shape.lift_le_bot a2).1 a3; exact .mk .rfl .bot .bot (.bot <| .bot .sort)
+    | cons h1 h2 h3 h4 ih =>
+      cases h with simp [Valuation.push] at a1 a2
+      | zero =>
+        exact ⟨_, _, _, a2, a3, .bvar a1 (Nat.le_refl _) (by rw [Shape.lift_self]; exact .rfl),
+          (LE_Interp.lift a1).2 h3.weak, (Shape.HasType.lift a1).2 h4⟩
+      | succ h =>
+        have ⟨_, _, _, le, h1, h2, h3, h4⟩ := ih h a1 a3
+        exact ⟨_, _, _, le, h1, h2.weak, h3.weak, h4⟩
+  | symm _ ih =>
+    refine ⟨(ih W).1.symm, fun h => ?_⟩
+    have ⟨_, _, _, le, a1, a2, a3⟩ := (ih W).2 ((ih W).1.2 h)
+    exact ⟨_, _, _, le, a1, (ih W).1.1 a2, a3⟩
+  | trans _ _ _ _ ih1 ih2 =>
+    refine ⟨(ih1 W).1.trans (ih2 W).1, fun h => ?_⟩
+    have ⟨_, _, _, le, a1, a2, a3⟩ := (ih2 W).2 ((ih1 W).1.1 h)
+    exact ⟨_, _, _, le, a1, (ih1 W).1.2 a2, a3⟩
+  | @sort _ l =>
+    refine ⟨.rfl, fun h => ?_⟩
+    generalize eq : SExpr.sort l = M at h
+    induction h with cases eq
+    | bot => exact .mk .rfl .bot .bot (.bot <| .bot .sort)
+    | sort h1 => exact .mk h1 (.sort .rfl) (.sort .rfl) .sort
+  | @const c _ _ ls =>
+    refine ⟨.rfl, fun h => ?_⟩
+    generalize eq : SExpr.const c ls = M at h
+    induction h with cases eq
+    | bot => exact .mk .rfl .bot .bot (.bot <| .bot .sort)
+  | appDF _ _ _ _ _ ihA ihB ih1 ih2 ih3 =>
+    by_cases hm : m = .bot; · exact hm ▸ sound_bot
+    refine ⟨⟨fun h => ?_, fun h => ?_⟩, fun h => ?_⟩ <;>
+      cases h with | bot => cases hm rfl | app h1 h2 h3
+    · exact .app ((ih1 W).1.1 h1) ((ih2 W).1.1 h2) h3
+    · exact .app ((ih1 W).1.2 h1) ((ih2 W).1.2 h2) h3
+    · exact sound_app (ih1 W).2 (hsort (ih3 W).2) (.app h1 h2 h3)
+  | @lamDF _ _ _ _ body body' B _ _ ih1 ih2 =>
+    by_cases hm : m = .bot; · exact hm ▸ sound_bot
+    refine ⟨⟨fun h => ?_, fun h => ?_⟩, fun h => ?_⟩ <;>
+      cases h with | bot => cases hm rfl | @lam _ n a _ f _ m h1 h2 h3 h4
+    · refine .lam ((ih1 W).1.1 h1) h2 (fun _ h => ?_) h4
+      exact (ih2 (W.cons (hsort (ih1 W).2) h1 h)).1.1 (h3 _ h)
+    · refine .lam ((ih1 W).1.2 h1) h2 (fun _ h => ?_) h4
+      exact (ih2 (W.cons (hsort (ih1 W).2) ((ih1 W).1.2 h1) h)).1.2 (h3 _ h)
+    · cases m with simp [Shape.LE.def] at h4 | bot => cases hm rfl | lam f'
+      have ⟨m', a', le, a1, a2, a3⟩ := hsort (ih1 W).2 h1
+      suffices ∃ n', n ≤ n' ∧ ∃ f' b : ShapeFun n', ShapeFun.LE (ShapeFun.lift Shape.lift f) f' ∧
+          Shape.HasDom f' a.lift ∧ Shape.HasDom b a.lift ∧ ∀ x, x.HasType a.lift →
+          LE_Interp (ρ.push x) (f'.app x) body ∧ LE_Interp (ρ.push x) (b.app x) B ∧
+          (f'.app x).HasType (b.app x) by
+        have ⟨n', le', f₁, b, a1, a2, a3, a4⟩ := this; simp [forall_and] at a4
+        have h1' := (LE_Interp.lift le').2 h1
+        exact ⟨_+1, .lam f₁, _, Nat.succ_le_succ le',
+          .trans (t := Shape.lift (n := _+1) (.lam f)) (Shape.lift_mono (Shape.LE.def.2 h4)) a1,
+          .lam h1' a2 a4.1 .rfl, .forallE h1' h1' a3 a4.2.1 .rfl,
+          .lam ⟨⟨a3, fun _ h => (a4.2.2 _ h).isType⟩, a2, a4.2.2⟩⟩
+      replace h3 (p) (h : p ∈ f) : p.1.HasType a ∧ LE_Interp (ρ.push p.1) p.2 body :=
+        have := Shape.HasDom.def.1 h2 _ _ h; ⟨this, (ShapeFun.app_of_mem h) ▸ h3 _ this⟩
+      have ⟨n', le, H⟩ : ∃ n', n ≤ n' ∧ ∀ k, n' ≤ k → ∃ f' b : ShapeFun k,
+          f'.map Prod.fst = f.map (·.1.lift) ∧ b.map Prod.fst = f.map (·.1.lift) ∧
+          ∀ x fx, (x, fx) ∈ f → ∃ f'x bx, (x.lift, f'x) ∈ f' ∧ (x.lift, bx) ∈ b ∧
+          fx.lift ≤ f'x ∧ LE_Interp (ρ.push x) f'x body ∧ LE_Interp (ρ.push x) bx B ∧
+          f'x.HasType bx := by
+        clear h2 h4
+        induction f with
+        | nil => exact ⟨_, Nat.le_refl _, fun _ _ => ⟨[], [], by simp⟩⟩
+        | cons p _ ih; let (x, fx) := p
+        simp only [List.mem_cons, forall_eq_or_imp] at h3
+        have ⟨k₁, le1, H1⟩ := ih h3.2
+        have ⟨m', f'x, bx, le, b1, b2, b3, b4⟩ :=
+          (ih2 (W.cons (hsort (ih1 W).2) h1 h3.1.1)).2 h3.1.2
+        refine ⟨k₁.max m', Nat.le_trans le (Nat.le_max_right ..), fun k le' => ?_⟩
+        have ⟨le₁, le₂⟩ := Nat.max_le.1 le'
+        have ⟨f', b, a1, a2, a3⟩ := H1 _ le₁
+        refine ⟨(x.lift, f'x.lift) :: f', (x.lift, bx.lift) :: b, ?_⟩
+        simp [or_imp, forall_and, *]
+        exact ⟨.inl (.inl ⟨Shape.lift_lift (.inl le) ▸ Shape.lift_mono b1,
+          (LE_Interp.lift le₂).2 b2, (LE_Interp.lift le₂).2 b3,
+          (Shape.HasType.lift le₂).2 b4⟩), by grind⟩
+      have ⟨f', b, a1, a2, a3⟩ := H _ (Nat.le_refl _)
+      refine ⟨_, le, f', b, ShapeFun.LE.def.2 fun _ _ h => ?_, ?_, ?_, fun x h => ?_⟩
+      simp [ShapeFun.lift] at h; obtain ⟨_, _, h, rfl, rfl⟩ := h
+      · have ⟨_, _, b1, _, b3, _⟩ := a3 _ _ h; exact ⟨_, _, b1, .rfl, b3⟩
+      · refine Shape.HasDom.def.2 fun _ _ h => ?_
+        obtain ⟨⟨_, _⟩, h1, ⟨⟩⟩ := List.mem_map.1 <| a1 ▸ List.mem_map.2 ⟨_, h, rfl⟩
+        exact (Shape.HasType.lift le).2 <| Shape.HasDom.def.1 h2 _ _ h1
+      · refine Shape.HasDom.def.2 fun _ _ h => ?_
+        obtain ⟨⟨_, _⟩, h1, ⟨⟩⟩ := List.mem_map.1 <| a2 ▸ List.mem_map.2 ⟨_, h, rfl⟩
+        exact (Shape.HasType.lift le).2 <| Shape.HasDom.def.1 h2 _ _ h1
+      · have ⟨x₁, _, b1, b2, rfl⟩ := ShapeFun.app_eq f' x
+        obtain ⟨⟨_, _⟩, b3, ⟨⟩⟩ := List.mem_map.1 <| a1 ▸ List.mem_map.2 ⟨_, b2, rfl⟩
+        have ⟨x₂, _, b1', b2', rfl⟩ := ShapeFun.app_eq b x
+        obtain ⟨⟨_, _⟩, b3', ⟨⟩⟩ := List.mem_map.1 <| a2 ▸ List.mem_map.2 ⟨_, b2', rfl⟩
+        have ⟨_, _, c1, c2, c3, c4, c5, c6⟩ := a3 _ _ b3
+        cases (ShapeFun.uniq_l b2 c1 .rfl .rfl).2
+        refine ⟨?_, ?_, ?_⟩
+        · exact c4.mono_l <| (Valuation.LE.push' le (Nat.le_refl _)).2
+            ⟨.rfl, (Shape.lift_self (s := x)).symm ▸ b1⟩
+        · have ⟨_, _, _, c2, _, _, c5, _⟩ := a3 _ _ b3'
+          cases (ShapeFun.uniq_l b2' c2 .rfl .rfl).2
+          exact c5.mono_l <| (Valuation.LE.push' le (Nat.le_refl _)).2
+            ⟨.rfl, (Shape.lift_self (s := x)).symm ▸ b1'⟩
+        · refine .mono_r (ShapeFun.app_of_mem c2 ▸ ShapeFun.app_mono_r b1) ?_ c6
+          have ⟨_, _, _, c2, _, _, c5, c6⟩ := a3 _ _ b3'
+          cases (ShapeFun.uniq_l b2' c2 .rfl .rfl).2
+          exact c6.isType
+  | @forallEDF _ A _ _ body body' _ _ _ ih1 ih2 =>
+    by_cases hm : m = .bot; · exact hm ▸ sound_bot
+    refine ⟨⟨fun h => ?_, fun h => ?_⟩, fun h => ?_⟩ <;>
+      cases h with | bot => cases hm rfl | @forallE _ n b₀ _ b f _ m h1 h2 h3 h4 h5
+    · refine .forallE ((ih1 W).1.1 h1) ((ih1 W).1.1 h2) h3 (fun _ h => ?_) h5
+      exact (ih2 (W.cons (hsort (ih1 W).2) h2 h)).1.1 (h4 _ h)
+    · refine .forallE ((ih1 W).1.2 h1) ((ih1 W).1.2 h2) h3 (fun _ h => ?_) h5
+      exact (ih2 (W.cons (hsort (ih1 W).2) ((ih1 W).1.2 h2) h)).1.2 (h4 _ h)
+    · cases m with simp [Shape.LE.def] at h5 | bot => cases hm rfl | forallE b' f'
+      have ⟨b₁, a1, a2, a3⟩ := hsort (ih1 W).2 h2
+      suffices ∃ n', n ≤ n' ∧ ∃ f' : ShapeFun n', ShapeFun.LE (ShapeFun.lift Shape.lift f) f' ∧
+          Shape.HasDom f' b.lift ∧ ∀ x, x.HasType b.lift →
+          LE_Interp (ρ.push x) (f'.app x) body ∧ (f'.app x).HasType .sort by
+        have ⟨n', le', f₁, b1, b2, b3⟩ := this; simp [forall_and] at b3
+        have hJ := Shape.Join.mk (h1.compat h2)
+        have ⟨m', b₂, le, c1, c2, c3⟩ := hsort (ih1 W).2 (h1.join hJ h2)
+        have le₁ := Nat.le_max_right n' m'
+        have le₂ := Nat.le_max_left n' m'
+        have hJ' := (Shape.Join.lift le).2 hJ
+        have hJ₂ := (Shape.Join.lift (Nat.le_trans le le₁)).2 hJ
+        have b2' := Shape.lift_lift (.inl le') ▸ (Shape.HasDom.lift le₂).2 b2
+        refine ⟨n'.max m'+1, .forallE .., _, Nat.succ_le_succ (Nat.le_trans le le₁),
+          Shape.LE.def.2 ⟨
+            (Shape.lift_mono h5.1).trans (hJ₂.le.1.trans
+              (Shape.lift_lift (.inl le) ▸ Shape.lift_mono c1)),
+            .trans (ShapeFun.lift_mono h5.2)
+              (ShapeFun.lift_lift (.inl le') ▸ ShapeFun.lift_mono b1)⟩,
+          .forallE ((LE_Interp.lift le₁).2 c2)
+            ((LE_Interp.lift le₂).2 <| (LE_Interp.lift le').2 h2)
+            ((Shape.HasDom.lift le₂).2 b2) (fun x h => ?_) .rfl,
+          .sort .rfl,
+          .forallE ⟨.mono (Shape.lift_mono <| hJ'.le.2.trans c1)
+            (Shape.lift_sort ▸ (Shape.HasType.lift le₁).2 c3)
+            ((Shape.lift_lift (.inl le)).symm ▸ b2'), fun x h => ?_⟩⟩
+        · refine have ⟨_, _, d1, d2, d3⟩ := ShapeFun.app_eq ..; d3 ▸ ?_
+          simp [ShapeFun.lift] at d2; obtain ⟨_, _, d2, rfl, rfl⟩ := d2
+          have := ShapeFun.app_of_mem d2 ▸ b3.1 _ (Shape.HasDom.def.1 b2 _ _ d2)
+          refine (LE_Interp.lift le₂).2 <| this.mono_l ?_
+          exact (Valuation.LE.push' le₂ (Nat.le_refl _)).2 ⟨.rfl, Shape.lift_self ▸ d1⟩
+        · have ⟨y, d1, d2, d3⟩ := b2' x
+          refine have ⟨_, _, e1, e2, e3⟩ := ShapeFun.app_eq _ y; have d3' := e3 ▸ d3; ?_
+          simp [ShapeFun.lift] at e2; obtain ⟨_, _, e2, rfl, rfl⟩ := e2
+          refine .mono_l (ShapeFun.app_mono_r d1) d3 <|
+            e3 ▸ Shape.lift_sort.symm ▸ (Shape.HasType.lift le₂).2 ?_
+          exact ShapeFun.app_of_mem e2 ▸ b3.2 _ (Shape.HasDom.def.1 b2 _ _ e2)
+      replace h4 (p) (h : p ∈ f) : p.1.HasType b ∧ LE_Interp (ρ.push p.1) p.2 body :=
+        have := Shape.HasDom.def.1 h3 _ _ h; ⟨this, (ShapeFun.app_of_mem h) ▸ h4 _ this⟩
+      have ⟨n', le, H⟩ : ∃ n', n ≤ n' ∧ ∀ k, n' ≤ k → ∃ f' : ShapeFun k,
+          f'.map Prod.fst = f.map (·.1.lift) ∧
+          ∀ x fx, (x, fx) ∈ f → ∃ f'x, (x.lift, f'x) ∈ f' ∧
+          fx.lift ≤ f'x ∧ LE_Interp (ρ.push x) f'x body ∧ f'x.HasType .sort := by
+        clear h3 h5
+        induction f with
+        | nil => exact ⟨_, Nat.le_refl _, fun _ _ => ⟨[], by simp⟩⟩
+        | cons p _ ih; let (x, fx) := p
+        simp only [List.mem_cons, forall_eq_or_imp] at h4
+        have ⟨k₁, le1, H1⟩ := ih h4.2
+        have ⟨m', f'x, bx, le, b1, b2, b3, b4⟩ :=
+          (ih2 (W.cons (hsort (ih1 W).2) h2 h4.1.1)).2 h4.1.2
+        refine ⟨k₁.max m', Nat.le_trans le (Nat.le_max_right ..), fun k le' => ?_⟩
+        have ⟨le₁, le₂⟩ := Nat.max_le.1 le'
+        have ⟨f', a1, a2⟩ := H1 _ le₁
+        refine ⟨(x.lift, f'x.lift) :: f', ?_⟩
+        replace b4 : f'x.HasType .sort := by
+          cases b3 with
+          | sort h => exact .mono_r h .sort b4
+          | bot => cases b4.bot_r; exact .bot .sort
+        simp [or_imp, forall_and, *]
+        exact ⟨.inl ⟨Shape.lift_lift (.inl le) ▸ Shape.lift_mono b1, (LE_Interp.lift le₂).2 b2,
+          Shape.lift_sort ▸ (Shape.HasType.lift le₂).2 b4⟩, by grind⟩
+      have ⟨f', a1, a2⟩ := H _ (Nat.le_refl _)
+      refine ⟨_, le, f', ShapeFun.LE.def.2 fun _ _ h => ?_, ?_, fun x h => ?_⟩
+      · simp [ShapeFun.lift] at h; obtain ⟨_, _, h, rfl, rfl⟩ := h
+        have ⟨_, b1, b2, _⟩ := a2 _ _ h; exact ⟨_, _, b1, .rfl, b2⟩
+      · refine Shape.HasDom.def.2 fun _ _ h => ?_
+        obtain ⟨⟨_, _⟩, h1, ⟨⟩⟩ := List.mem_map.1 <| a1 ▸ List.mem_map.2 ⟨_, h, rfl⟩
+        exact (Shape.HasType.lift le).2 <| Shape.HasDom.def.1 h3 _ _ h1
+      · have ⟨x₁, _, b1, b2, rfl⟩ := ShapeFun.app_eq f' x
+        obtain ⟨⟨_, _⟩, b3, ⟨⟩⟩ := List.mem_map.1 <| a1 ▸ List.mem_map.2 ⟨_, b2, rfl⟩
+        have ⟨_, c1, c2, c3, c4⟩ := a2 _ _ b3
+        cases (ShapeFun.uniq_l b2 c1 .rfl .rfl).2
+        refine ⟨c3.mono_l ?_, c4⟩
+        exact (Valuation.LE.push' le (Nat.le_refl _)).2 ⟨.rfl, Shape.lift_self ▸ b1⟩
+  | defeqDF _ _ ih1 ih2 =>
+    refine ⟨(ih2 W).1, fun h => ?_⟩
+    have ⟨_, _, _, le, h1, h2, h3, h4⟩ := (ih2 W).2 h
+    exact ⟨_, _, _, le, h1, h2, (ih1 W).1.1 h3, h4⟩
+  | beta _ _ _ ih1 ih2 ih3 =>
+    by_cases hm : m = .bot; · exact hm ▸ sound_bot
+    refine ⟨⟨fun h => ?_, fun h => ?_⟩, (ih3 W).2⟩
+    · cases h with | bot => cases hm rfl | app h1 h2 h3
+      cases h1 with | bot => cases hm (Shape.le_bot.1 h3) | lam h4 h5 h6 h7
+      have ⟨_, _, a1, a2, a3, a4⟩ := (ih2 W).2 h2
+      refine have ⟨_, b1, b2, b3⟩ := h5 _; LE_Interp.inst.2 ⟨_, _, ?_, h2.mono b1⟩
+      exact (h6 _ b2).mono <| .trans h3 <| .trans (Shape.app_mono_l h7 _) b3
+    · have ⟨n', _, h1, h2⟩ := LE_Interp.inst.1 h
+      have ⟨_, _, _, le, a1, a2, a3, a4⟩ :=
+        (ih2 W).2 <| (LE_Interp.lift (Nat.le_max_right n n')).2 h2
+      have le' := Nat.max_le.1 le
+      refine (LE_Interp.lift le'.1).1 <|
+        .app (.lam a3 ((Shape.HasDom.single (y := m.lift)).2 a4) (fun _ h => ?_) .rfl) a2 ?_
+      · simp [ShapeFun.single_app]; split <;> [skip; exact .bot]
+        refine (LE_Interp.lift le'.1).2 <| h1.mono_l ?_
+        refine (Valuation.LE.push' le'.2 (Nat.le_refl _)).2
+          ⟨.rfl, .trans (Shape.lift_lift (.inl (Nat.le_max_right ..)) ▸ a1) ?_⟩
+        rwa [Shape.lift_self]
+      · rw [Shape.app, ShapeFun.single_app, if_pos .rfl]; exact .rfl
+  | @eta _ e _ _ _ _ ih1 ih2 =>
+    by_cases hm : m = .bot; · exact hm ▸ sound_bot
+    refine ⟨⟨fun h => ?_, fun h => ?_⟩, (ih2 W).2⟩
+    · have ⟨_, _, t, le, h1, h2, h3, h4⟩ := (ih2 W).2 h
+      have ht : t ≠ .bot := fun h => by
+        subst h; cases h4.bot_r; cases hm ((Shape.lift_le_bot le).1 h1)
+      cases h2 with
+      | bot => cases hm ((Shape.lift_le_bot le).1 h1)
+      | @lam _ _ _ _ f' _ _ a1 a2 a3 a4
+      cases h3 with | bot => cases ht rfl | @forallE _ _ _ _ _ _ _ m₁ b1 b2 b3 b4 b5
+      cases t with simp [Shape.LE.def] at b5 | bot => cases ht rfl | forallE a' b'
+      cases h4.unfold with | bot => cases hm ((Shape.lift_le_bot le).1 h1) | @lam _ f _ _ d1
+      have : ∀ x y, (x, y) ∈ f' → LE_Interp (ρ.push x) y (e.lift.app (SExpr.bvar 0)) := by
+        intro x y h
+        have hy : y ≠ .bot := sorry
+        have := ShapeFun.app_of_mem h ▸ a3 x (Shape.HasDom.def.1 a2 _ _ h)
+        cases this with | bot => cases hy rfl | app c1 c2 c3
+        have := LE_Interp.weak_iff.1 c1
+        have ⟨k, le₁, le₂, c2⟩ := LE_Interp.bvar_iff.1 c2
+        sorry
+      sorry
+    · have ⟨_, m', f, le, a1, a2, a3, a4⟩ := (ih1 W).2 h
+      have hf : f ≠ .bot := fun h => by
+        subst h; cases a4.bot_r; cases hm ((Shape.lift_le_bot le).1 a1)
+      cases a3 with | bot => cases hf rfl | @forallE _ _ _ _ _ _ _ m₁ b1 b2 b3 b4 b5
+      cases m₁ with simp [Shape.LE.def] at b5 | bot => cases hf rfl | forallE
+      cases a4.unfold with | bot => cases hm ((Shape.lift_le_bot le).1 a1) | lam d1
+      refine (LE_Interp.lift le).1 <| .lam (b1.mono b5.1) d1.2.1 (fun _ h => ?_) a1
+      exact .app a2.weak (.bvar (Nat.le_refl _) (Nat.le_refl _) .rfl) .rfl
+  | proofIrrel _ _ _ ih1 ih2 ih3 =>
+    refine ⟨⟨fun h => ?_, fun h => ?_⟩, (ih2 W).2⟩
+    · sorry
+    · sorry
+  | extra => sorry
+
 structure LogRelBase (Γ : List SExpr) (n : Nat) where
   DefEq' (M N A : SExpr) (m a : Shape n) : Prop
 
 def LogRelBase.DefEq (R : LogRelBase Γ n) (M N A : SExpr) (m a : Shape n) : Prop :=
   Shape.HasType m a ∧ Γ ⊢ M ≡ N : A
+    ∧ LE_Interp .nil m M ∧ LE_Interp .nil m N ∧ LE_Interp .nil a A
     -- ∧ CheckType Γ M A u ∧ CheckType Γ N A u ∧ InferTypeS Γ A (.sort u)
     ∧ R.DefEq' M N A m a
 
 structure LogRel (Γ : List SExpr) (n : Nat) extends LogRelBase Γ n where
   isType : toLogRelBase.DefEq M N A m a → Γ ⊢ A ≡ A : .sort u → DefEq' A A (.sort u) a .sort
+  sort : DefEq' (.sort u) (.sort u) (.sort u.succ) .sort .sort
   left : DefEq' M N A m a → DefEq' M M A m a
   symm : DefEq' M N A m a → DefEq' N M A m a
   trans : DefEq' M₁ M₂ A m a → DefEq' M₂ M₃ A m a → DefEq' M₁ M₃ A m a
   defeqDF : toLogRelBase.DefEq A B (.sort u) a .sort →
     DefEq' M N A m a → DefEq' M N B m a
-  mono'_2 : m.HasType a → m ≤ m' → a ≤ a' →
+  mono_2 : m.HasType a → m ≤ m' → a ≤ a' →
     toLogRelBase.DefEq A A (.sort u) a' .sort → DefEq' M N A m' a' → DefEq' M N A m a
-  mono'_r_1 : m.HasType a → a ≤ a' →
+  mono_r_1 : m.HasType a → a ≤ a' →
     toLogRelBase.DefEq A A (.sort u) a' .sort → DefEq' M N A m a → DefEq' M N A m a'
+  join : m₁ ≠ .bot → m₂ ≠ .bot → m₁.Compat m₂ →
+    toLogRelBase.DefEq M N A m₁ a → toLogRelBase.DefEq M N A m₂ a → DefEq' M N A (m₁.join m₂) a
 
 theorem LogRelBase.DefEq.isType {R : LogRel Γ n}
     (H : R.DefEq M N A m a) : ∃ u, R.DefEq A A (.sort u) a .sort :=
-  have ⟨h1, h2, _⟩ := H
+  have ⟨h1, h2, _, _, h5, _⟩ := H
   have ⟨_, h2'⟩ := h2.isType
-  ⟨_, h1.isType, h2', R.isType H h2'⟩
+  ⟨_, h1.isType, h2', h5, h5, .sort .rfl, R.isType H h2'⟩
 
 theorem LogRelBase.DefEq.mono_2 {R : LogRel Γ n}
     (hm : m.HasType a) (le1 : m ≤ m') (le2 : a ≤ a') (hA : R.DefEq A A (.sort u) a' .sort) :
     R.DefEq M N A m' a' → R.DefEq M N A m a
-  | ⟨_, h2, h3⟩ => ⟨hm, h2, R.mono'_2 hm le1 le2 hA h3⟩
+  | ⟨_, h2, h3, h4, h5, h6⟩ =>
+    ⟨hm, h2, h3.mono le1, h4.mono le1, h5.mono le2, R.mono_2 hm le1 le2 hA h6⟩
 
 theorem LogRelBase.DefEq.mono_l {R : LogRel Γ n}
-    (hm : m.HasType .sort) (le : m ≤ m') (H : R.DefEq M N A m' .sort) : R.DefEq M N A m .sort :=
+    (hm : m.HasType a) (le : m ≤ m') (H : R.DefEq M N A m' a) : R.DefEq M N A m a :=
   let ⟨_, h⟩ := H.isType; h.mono_2 hm le .rfl H
 
 theorem LogRelBase.DefEq.mono_r_1 {R : LogRel Γ n}
     (ha : a ≤ a') (hA : R.DefEq A A (.sort u) a' .sort) : R.DefEq M N A m a → R.DefEq M N A m a'
-  | ⟨ht, h2, h3⟩ => ⟨.mono_r ha hA.1 ht, h2, R.mono'_r_1 ht ha hA h3⟩
+  | ⟨ht, h2, h3, h4, _, h6⟩ => ⟨.mono_r ha hA.1 ht, h2, h3, h4, hA.2.2.1, R.mono_r_1 ht ha hA h6⟩
 
 theorem LogRelBase.DefEq.mono_r_2 {R : LogRel Γ n}
     (ht : m.HasType a) (ha : a ≤ a') (H : R.DefEq M N A m a') : R.DefEq M N A m a :=
   let ⟨_, h⟩ := H.isType; h.mono_2 ht .rfl ha H
 
 theorem LogRelBase.DefEq.left {R : LogRel Γ n} : R.DefEq M N A m a → R.DefEq M M A m a
-  | ⟨h1, h2, h6⟩ => ⟨h1, h2.hasType.1, R.left h6⟩
+  | ⟨h1, h2, h3, _, h5, h6⟩ => ⟨h1, h2.hasType.1, h3, h3, h5, R.left h6⟩
 
 theorem LogRelBase.DefEq.symm {R : LogRel Γ n} : R.DefEq M N A m a → R.DefEq N M A m a
-  | ⟨h1, h2, h6⟩ => ⟨h1, h2.symm, R.symm h6⟩
+  | ⟨h1, h2, h3, h4, h5, h6⟩ => ⟨h1, h2.symm, h4, h3, h5, R.symm h6⟩
 
 theorem LogRelBase.DefEq.trans {R : LogRel Γ n} :
     R.DefEq M₁ M₂ A m a → R.DefEq M₂ M₃ A m a → R.DefEq M₁ M₃ A m a
-  | ⟨a1, a2, a3⟩, ⟨_, b2, b3⟩ => ⟨a1, a2.trans b2, R.trans a3 b3⟩
+  | ⟨a1, a2, a3, _, a5, a6⟩, ⟨_, b2, _, b4, _, b6⟩ => ⟨a1, a2.trans b2, a3, b4, a5, R.trans a6 b6⟩
+
+theorem LogRelBase.DefEq.join {R : LogRel Γ n} (hJ : m₁.Join m₂ m)
+    (h1 : R.DefEq M N A m₁ a) (h2 : R.DefEq M N A m₂ a) : R.DefEq M N A m a := by
+  have ⟨_, h2'⟩ := h2.isType
+  by_cases c1 : m₁ = .bot
+  · exact .mono_2 (.join hJ h1.1 h2.1) ((hJ _).2 ⟨c1 ▸ Shape.bot_le, .rfl⟩) .rfl h2' h2
+  by_cases c2 : m₂ = .bot
+  · exact .mono_2 (.join hJ h1.1 h2.1) ((hJ _).2 ⟨.rfl, c2 ▸ Shape.bot_le⟩) .rfl h2' h1
+  let ⟨a1, a2, a3, a4, a5, _⟩ := h1; let ⟨b1, _, b3, b4, _⟩ := h2
+  refine ⟨a1.join hJ b1, a2, a3.join hJ b3, a4.join hJ b4, a5, ?_⟩
+  have ⟨_, h⟩ := h1.isType
+  refine R.mono_2 (a1.join hJ b1) (Shape.Join.iff.1 hJ).2.2 .rfl h (R.join c1 c2 hJ.compat h1 h2)
 
 theorem LogRelBase.DefEq.defeqDF {R : LogRel Γ n}
     (hA : R.DefEq A B (.sort u) a .sort) : R.DefEq M N A m a → R.DefEq M N B m a
-  | ⟨ht, h2, h6⟩ =>
-    let ⟨_, a2, _⟩ := hA
-    -- have ⟨_, a4⟩ := R.sort_r a3
+  | ⟨ht, h2, h3, h4, _, h6⟩ =>
+    let ⟨_, a2, _, a4, _⟩ := hA
     have ⟨_, b1⟩ := a2.isType
-    ⟨ht, .defeqDF (b1.defeqDF a2) h2, R.defeqDF hA h6⟩
+    ⟨ht, .defeqDF (b1.defeqDF a2) h2, h3, h4, a4, R.defeqDF hA h6⟩
+
+theorem LogRelBase.DefEq.sort {R : LogRel Γ n} :
+    R.DefEq (.sort u) (.sort u) (.sort u.succ) .sort .sort :=
+  ⟨.sort, .sort, .sort .rfl, .sort .rfl, .sort .rfl, R.sort⟩
 
 theorem LogRel.mono_r {R : LogRel Γ n}
     (ht : m.HasType a) (hA : R.DefEq A A (.sort u) a' .sort) (ha : a ≤ a') :
     R.DefEq M N A m a ↔ R.DefEq M N A m a' := ⟨.mono_r_1 ha hA, .mono_r_2 ht ha⟩
 
-def TypeEq0.DefEqTy (Γ : List SExpr) (M N : SExpr) (m : Shape 0) : Prop :=
+def LR0.DefEqTy (Γ : List SExpr) (M N : SExpr) (m : Shape 0) : Prop :=
   match m with
   | .bot => True
-  | .sort => ∃ u, WHRedS Γ M (.sort u) ∧ WHRedS Γ N (.sort u)
+  | .sort => ∃ u, Γ ⊢ M ⤳* .sort u ∧ Γ ⊢ N ⤳* .sort u
 
-def TypeEqS.DefEqTy (IH : LogRel Γ n)
+def LRS.DefEqTy (IH : LogRel Γ n)
     (Γ : List SExpr) (M N : SExpr) (m : Shape (n+1)) : Prop :=
   match m with
   | .bot => True
-  | .sort => ∃ u, WHRedS Γ M (.sort u) ∧ WHRedS Γ N (.sort u)
+  | .sort => ∃ u, Γ ⊢ M ⤳* .sort u ∧ Γ ⊢ N ⤳* .sort u
   | .forallE m₁ m₂ =>
-    ∃ M₁ M₂ N₁ N₂, WHRedS Γ M (.forallE M₁ M₂) ∧ WHRedS Γ N (.forallE N₁ N₂) ∧
+    ∃ M₁ M₂ N₁ N₂, Γ ⊢ M ⤳* .forallE M₁ M₂ ∧ Γ ⊢ N ⤳* .forallE N₁ N₂ ∧
     ∃ u v, IH.DefEq M₁ N₁ (.sort u) m₁ .sort ∧ M₁::Γ ⊢ M₂ ≡ N₂ : sort v ∧
     (∀ {{a b p}}, IH.DefEq a b M₁ p m₁ →
       IH.DefEq (M₂.inst a) (M₂.inst b) (.sort v) (ShapeFun.app m₂ p) .sort ∧
@@ -536,73 +1142,72 @@ def TypeEqS.DefEqTy (IH : LogRel Γ n)
       IH.DefEq (M₂.inst a) (N₂.inst a) (.sort v) (ShapeFun.app m₂ p) .sort)
   | _ => False
 
-def TypeEqS.DefEqForall (IH : LogRel Γ n) (M N A₁ A₂ : SExpr) (m : Shape (n+1))
+def LRS.DefEqForall (IH : LogRel Γ n) (M N A₁ A₂ : SExpr) (m : Shape (n+1))
     (a₁ : Shape n) (a₂ : ShapeFun n) : Prop :=
   match m with
   | .bot => True
   | .lam m =>
     (∀ {{a b p}}, IH.DefEq a b A₁ p a₁ →
-      IH.DefEq (M.inst a) (M.inst b) (A₂.inst a) (ShapeFun.app m p) (ShapeFun.app a₂ p) ∧
-      IH.DefEq (N.inst a) (N.inst b) (A₂.inst a) (ShapeFun.app m p) (ShapeFun.app a₂ p)) ∧
+      IH.DefEq (M.app a) (M.app b) (A₂.inst a) (ShapeFun.app m p) (ShapeFun.app a₂ p) ∧
+      IH.DefEq (N.app a) (N.app b) (A₂.inst a) (ShapeFun.app m p) (ShapeFun.app a₂ p)) ∧
     (∀ {{a p}}, IH.DefEq a a A₁ p a₁ →
-      IH.DefEq (M.inst a) (N.inst a) (A₂.inst a) (ShapeFun.app m p) (ShapeFun.app a₂ p))
+      IH.DefEq (M.app a) (N.app a) (A₂.inst a) (ShapeFun.app m p) (ShapeFun.app a₂ p))
   | _ => False
 
-def TypeEqS.DefEq' (IH : LogRel Γ n) (M N A : SExpr) (m a : Shape (n+1)) : Prop :=
+def LRS.DefEq' (IH : LogRel Γ n) (M N A : SExpr) (m a : Shape (n+1)) : Prop :=
   match a with
   | .bot => True
-  | .sort => ∃ u, WHRedS Γ A (.sort u) ∧ DefEqTy IH Γ M N m
-  | .forallE a₁ a₂ => ∃ A₁ A₂ u v, WHRedS Γ A (.forallE A₁ A₂) ∧
+  | .sort => ∃ u, Γ ⊢ A ⤳* .sort u ∧ DefEqTy IH Γ M N m
+  | .forallE a₁ a₂ => ∃ A₁ A₂ u v, Γ ⊢ A ⤳* .forallE A₁ A₂ ∧
     IH.DefEq A₁ A₁ (.sort u) a₁ .sort ∧ A₁::Γ ⊢ A₂ : sort v ∧
     (∀ {{a b p}}, IH.DefEq a b A₁ p a₁ →
       IH.DefEq (A₂.inst a) (A₂.inst b) (.sort v) (ShapeFun.app a₂ p) .sort) ∧
     DefEqForall IH M N A₁ A₂ m a₁ a₂
   | _ => False
 
-def TypeEq0.DefEq' (Γ : List SExpr) (M N A : SExpr) (m a : Shape 0) : Prop :=
+def LR0.DefEq' (Γ : List SExpr) (M N A : SExpr) (m a : Shape 0) : Prop :=
   match a with
   | .bot => True
-  | .sort => ∃ u, WHRedS Γ A (.sort u) ∧ DefEqTy Γ M N m
+  | .sort => ∃ u, Γ ⊢ A ⤳* .sort u ∧ DefEqTy Γ M N m
 
-def TypeEq0 : LogRel Γ 0 := by
-  refine {
-    DefEq' := TypeEq0.DefEq' Γ
-    isType {M N A m a u} h1 hA := ?_
-    left {M N A m a} h1 := ?_
-    symm {M N A m a} h1 := ?_
-    trans {M₁ M₂ A m a M₃} := ?_
-    defeqDF {A B u a M N m} hA := ?_
-    mono'_2 {m m' a a' A U M N} h1 hm ha hA := ?_
-    mono'_r_1 {a a' A U M N m} h1 le hA := ?_ }
-  · let ⟨h1, h2, h6⟩ := h1
-    simp [TypeEq0.DefEq'] at h6; split at h6
+def LR0 : LogRel Γ 0 where
+  DefEq' := LR0.DefEq' Γ
+  isType {M N A m a u} h1 hA := by
+    let ⟨h1, h2, _, _, _, h6⟩ := h1
+    simp [LR0.DefEq'] at h6; split at h6
     · exact ⟨_, .rfl, trivial⟩
     · obtain ⟨⟨v, h1⟩, h2⟩ := h6; exact ⟨_, .rfl, _, h1, h1⟩
-  · dsimp [TypeEq0.DefEq'] at h1 ⊢; split at h1
+  sort := ⟨_, .rfl, _, .rfl, .rfl⟩
+  left {M N A m a} h1 := by
+    dsimp [LR0.DefEq'] at h1 ⊢; split at h1
     · trivial
     · let ⟨_, h1, h3⟩ := h1; refine ⟨_, h1, ?_⟩
-      dsimp [TypeEq0.DefEqTy] at h3 ⊢; split at h3
+      dsimp [LR0.DefEqTy] at h3 ⊢; split at h3
       · trivial
       · let ⟨h1, h3, _⟩ := h3; exact ⟨h1, h3, h3⟩
-  · dsimp [TypeEq0.DefEq'] at h1 ⊢; split at h1
+  symm {M N A m a} h1 := by
+    dsimp [LR0.DefEq'] at h1 ⊢; split at h1
     · trivial
     · let ⟨_, h1, h3⟩ := h1; refine ⟨_, h1, ?_⟩
-      dsimp [TypeEq0.DefEqTy] at h3 ⊢; split at h3
+      dsimp [LR0.DefEqTy] at h3 ⊢; split at h3
       · trivial
       · let ⟨h1, h3, h4⟩ := h3; exact ⟨h1, h4, h3⟩
-  · dsimp [TypeEq0.DefEq']; split
+  trans {M₁ M₂ A m a M₃} := by
+    dsimp [LR0.DefEq']; split
     · simp
     · rintro ⟨_, a1, a2⟩ ⟨_, -, b2⟩; refine ⟨_, a1, ?_⟩
-      revert a2 b2; dsimp [TypeEq0.DefEqTy]; split
+      revert a2 b2; dsimp [LR0.DefEqTy]; split
       · simp
       · rintro ⟨_, a1, a2⟩ ⟨_, b1, b2⟩; cases a2.determ .sort b1 .sort; exact ⟨_, a1, b2⟩
-  · obtain ⟨A1, A2, A6⟩ := hA
-    dsimp [TypeEq0.DefEq']; split
+  defeqDF {A B u a M N m} hA := by
+    obtain ⟨A1, A2, _, _, _, A6⟩ := hA
+    dsimp [LR0.DefEq']; split
     · trivial
     · rintro ⟨u, a1, a2⟩
       let ⟨_, _, _, _, b3⟩ := A6
       exact ⟨_, b3, a2⟩
-  · obtain ⟨A1, A2, _, A3, A4⟩ := hA
+  mono_2 {m m' a a' A U M N} h1 hm ha hA := by
+    obtain ⟨A1, A2, _, A3, A4⟩ := hA
     cases h1.unfold with
     | bot h1 =>
       cases A1.unfold with
@@ -614,35 +1219,33 @@ def TypeEq0 : LogRel Γ 0 := by
       cases m' <;> cases hm
       cases a' <;> cases ha
       exact id
-  · obtain ⟨A1, A2, _, A3, A4⟩ := hA
+  mono_r_1 {a a' A U M N m} h1 le hA := by
+    obtain ⟨A1, A2, _, _, _, _, A3, A4⟩ := hA
     cases A1.unfold with
     | bot => cases Shape.le_bot.1 le; exact id
     | sort =>
       obtain rfl|rfl := Shape.le_sort.1 le <;> [rintro -; exact id]
       cases h1.unfold; have ⟨_, h, _⟩ := A4; exact ⟨_, h, ⟨⟩⟩
+  join {m₁ m₂ M N A a} ne1 _ _ h1 _ :=
+    match m₁ with | .bot => nomatch ne1 rfl | .sort => by cases m₂ <;> exact h1.2.2.2.2.2
 
-def TypeEqS (IH : LogRel Γ n) : LogRel Γ (n + 1) := by
-  refine {
-    DefEq' := TypeEqS.DefEq' IH
-    isType {M N A m a u} h1 hA := ?_
-    left {M N A m a} h1 := ?_
-    symm {M N A m a} h1 := ?_
-    trans {M₁ M₂ A m a M₃} := ?_
-    defeqDF {A B u a M N m} hA := ?_
-    mono'_2 {m m' a a' A U M N} h1 hm ha hA := ?_
-    mono'_r_1 {a a' A U M N m} h1 le hA := ?_ }
-  · let ⟨h1, h2, h6⟩ := h1
-    simp [TypeEqS.DefEq'] at h6; split at h6
+def LRS (IH : LogRel Γ n) : LogRel Γ (n + 1) where
+  DefEq' := LRS.DefEq' IH
+  isType {M N A m a u} h1 hA := by
+    let ⟨h1, h2, _, _, _, h6⟩ := h1
+    simp [LRS.DefEq'] at h6; split at h6
     · exact ⟨_, .rfl, trivial⟩
     · obtain ⟨⟨v, h1⟩, h2⟩ := h6; exact ⟨_, .rfl, _, h1, h1⟩
     · obtain ⟨_, _, h1, ⟨_, h2⟩, _, h3, h4, _⟩ := h6
       exact ⟨_, .rfl, _, _, _, _, h1, h1, _, _, h2, h3,
         fun _ _ _ a1 => ⟨h4 a1, h4 a1⟩, fun _ _ a1 => h4 a1⟩
     · cases h6
-  · dsimp [TypeEqS.DefEq'] at h1 ⊢; split at h1
+  sort := ⟨_, .rfl, _, .rfl, .rfl⟩
+  left {M N A m a} h1 := by
+    dsimp [LRS.DefEq'] at h1 ⊢; split at h1
     · trivial
     · let ⟨_, h1, h3⟩ := h1; refine ⟨_, h1, ?_⟩
-      dsimp [TypeEqS.DefEqTy] at h3 ⊢; split at h3
+      dsimp [LRS.DefEqTy] at h3 ⊢; split at h3
       · trivial
       · let ⟨h1, h3, _⟩ := h3; exact ⟨h1, h3, h3⟩
       · let ⟨_, _, _, _, h1, _, _, h3, h4, h4', h5, h6⟩ := h3
@@ -650,15 +1253,16 @@ def TypeEqS (IH : LogRel Γ n) : LogRel Γ (n + 1) := by
           fun a b p a1 => ⟨(h5 a1).1, (h5 a1).1⟩, fun a p a1 => (h5 a1).1⟩
       · cases h3
     · let ⟨_, _, _, _, h1, h3, h4, h5, h6⟩ := h1; refine ⟨_, _, _, _, h1, h3, h4, h5, ?_⟩
-      dsimp [TypeEqS.DefEqForall] at h6 ⊢; split at h6
+      dsimp [LRS.DefEqForall] at h6 ⊢; split at h6
       · trivial
       · exact ⟨fun a b p a1 => ⟨(h6.1 a1).1, (h6.1 a1).1⟩, fun a p a1 => (h6.1 a1).1⟩
       · cases h6
     · cases h1
-  · dsimp [TypeEqS.DefEq'] at h1 ⊢; split at h1
+  symm {M N A m a} h1 := by
+    dsimp [LRS.DefEq'] at h1 ⊢; split at h1
     · trivial
     · let ⟨_, h1, h3⟩ := h1; refine ⟨_, h1, ?_⟩
-      dsimp [TypeEqS.DefEqTy] at h3 ⊢; split at h3
+      dsimp [LRS.DefEqTy] at h3 ⊢; split at h3
       · trivial
       · let ⟨h1, h3, h4⟩ := h3; exact ⟨h1, h4, h3⟩
       · let ⟨B, F, B', F', h1, h2, _, _, h3, h4, h5, h6⟩ := h3
@@ -667,15 +1271,16 @@ def TypeEqS (IH : LogRel Γ n) : LogRel Γ (n + 1) := by
         · exact fun a p a1 => (h6 (.defeqDF h3.symm a1)).symm
       · cases h3
     · let ⟨_, _, _, _, h1, h2, h3, h4, h6⟩ := h1; refine ⟨_, _, _, _, h1, h2, h3, h4, ?_⟩
-      dsimp [TypeEqS.DefEqForall] at h6 ⊢; split at h6
+      dsimp [LRS.DefEqForall] at h6 ⊢; split at h6
       · trivial
       · exact ⟨fun a b p a1 => (h6.1 a1).symm, fun a p a1 => (h6.2 a1).symm⟩
       · cases h6
     · cases h1
-  · dsimp [TypeEqS.DefEq']; split
+  trans {M₁ M₂ A m a M₃} := by
+    dsimp [LRS.DefEq']; split
     · simp
     · rintro ⟨_, a1, a2⟩ ⟨_, -, b2⟩; refine ⟨_, a1, ?_⟩
-      revert a2 b2; dsimp [TypeEqS.DefEqTy]; split
+      revert a2 b2; dsimp [LRS.DefEqTy]; split
       · simp
       · rintro ⟨_, a1, a2⟩ ⟨_, b1, b2⟩; cases a2.determ .sort b1 .sort; exact ⟨_, a1, b2⟩
       · rintro ⟨B, F, B', F', a1', a2, u, v, a4, a4', a5, a6⟩
@@ -693,14 +1298,15 @@ def TypeEqS (IH : LogRel Γ n) : LogRel Γ (n + 1) := by
       cases a1.determ .forallE b1 .forallE
       cases a2.2.1.uniq_sort b2.2.1; cases a3.uniq_sort b3
       refine ⟨_, _, _, _, a1, a2, a3, a4, ?_⟩
-      revert a5 b5; dsimp [TypeEqS.DefEqForall]; split
+      revert a5 b5; dsimp [LRS.DefEqForall]; split
       · simp
       · intro ⟨a5, a6⟩ ⟨b5, b6⟩
         exact ⟨fun _ _ _ c1 => ⟨(a5 c1).1, (b5 c1).2⟩, fun _ _ c1 => (a6 c1).trans (b6 c1)⟩
       · nofun
     · nofun
-  · obtain ⟨A1, A2, A6⟩ := hA
-    dsimp [TypeEqS.DefEq']; split
+  defeqDF {A B u a M N m} hA := by
+    obtain ⟨A1, A2, _, _, _, A6⟩ := hA
+    dsimp [LRS.DefEq']; split
     · trivial
     · rintro ⟨u, a1, a2⟩
       let ⟨_, _, _, _, b3⟩ := A6
@@ -710,7 +1316,7 @@ def TypeEqS (IH : LogRel Γ n) : LogRel Γ (n + 1) := by
       cases a1.determ .forallE b2 .forallE
       refine ⟨_, _, _, _, b3, b4.symm.left, b4.2.1.defeqDF_l b4'.hasType.2,
         fun _ _ _ c1 => (b5 (.defeqDF b4.symm c1)).2, ?_⟩
-      revert a5; dsimp [TypeEqS.DefEqForall]; split
+      revert a5; dsimp [LRS.DefEqForall]; split
       · simp
       · refine fun ⟨d1, d2⟩ => ⟨fun _ _ _ c1 => ?_, fun _ _ c1 => ?_⟩ <;>
           have c2 := b4.symm.defeqDF c1
@@ -718,7 +1324,9 @@ def TypeEqS (IH : LogRel Γ n) : LogRel Γ (n + 1) := by
         · exact .defeqDF (b6 c2) (d2 c2)
       · nofun
     · nofun
-  · obtain ⟨A1, A2, _, A3, A4⟩ := hA
+  mono_2 {m m' a a' A U M N} h1 hm ha hA := by
+    stop
+    obtain ⟨A1, A2, _, _, _, _, A3, A4⟩ := hA
     cases h1.unfold with
     | bot h1 =>
       cases A1.unfold with
@@ -759,7 +1367,9 @@ def TypeEqS (IH : LogRel Γ n) : LogRel Γ (n + 1) := by
           ⟨.mono_2 h1 h2 h3 h4 a7, .mono_2 h1 h2 h3 h4 a8⟩
       · exact .mono_2 (.lam_app c3 d.1) (ShapeFun.app_mono_l hm _)
           (ShapeFun.app_mono_l ha.2 _) (a4 (.mono_r_1 ha.1 a2 d.left)) (a6 (.mono_r_1 ha.1 a2 d))
-  · obtain ⟨A1, A2, _, A3, A4⟩ := hA
+  mono_r_1 {a a' A U M N m} h1 le hA := by
+    stop
+    obtain ⟨A1, A2, _, _, _, _, A3, A4⟩ := hA
     cases A1.unfold with
     | bot => cases Shape.le_bot.1 le; exact id
     | sort =>
@@ -780,8 +1390,60 @@ def TypeEqS (IH : LogRel Γ n) : LogRel Γ (n + 1) := by
       · have ⟨_, c2, c3, eq⟩ := Shape.HasType.maximal a5 le.1 c1.1
         exact have h3 := .trans (ShapeFun.app_mono_l le.2 _) (ShapeFun.app_mono_r c3)
           .mono_r_1 h3 (A8 c1).1.left (eq ▸ B8 (.mono_2 c2 c3 le.1 A6.left c1))
+  join {m₁ m₂ M N A a} ne1 ne2 hC h1 h2 := by
+    cases h1.1.unfold with
+    | bot => cases ne1 rfl
+    | sort =>
+      cases m₂ with simp [Shape.Compat] at hC | bot => cases ne2 rfl | sort
+      exact h1.2.2.2.2.2
+    | forallE =>
+      cases m₂ with simp [Shape.Compat] at hC | bot => cases ne2 rfl | forallE
+      simp [Shape.join]
+      have hJ₁ := Shape.Join.mk hC.1; have hJ₂ := ShapeFun.Join.mk hC.2
+      have ⟨_, _, _, _, _, _, a1, _, _, _, _, a2, a3, _, _, a4, a5, a6, a7⟩ := h1
+      have ⟨_, _, _, _, _, _, b1, _, _, _, _, b2, b3, _, _, b4, b5, b6, b7⟩ := h2
+      cases a2.determ .forallE b2 .forallE; cases a3.determ .forallE b3 .forallE
+      cases a4.2.1.uniq_sort b4.2.1.symm
+      refine ⟨_, a1, _, _, _, _, a2, a3, _, _, a4.join hJ₁ b4, a5,
+        fun _ _ _ c1 => ⟨?_, ?_⟩, fun _ _ c1 => ?_⟩
+      · stop
+        have := a6 (c1.mono_r_2 _ hJ₁.le.1)
+        sorry
+      · sorry
+      · sorry
+    | lam _ => sorry
 
-def TypeEq (Γ : List SExpr) : LogRel Γ n :=
+def LR (Γ : List SExpr) : LogRel Γ n :=
   match n with
-  | 0 => TypeEq0
-  | _+1 => TypeEqS (TypeEq Γ)
+  | 0 => LR0
+  | _+1 => LRS (LR Γ)
+
+inductive LR.Subst : (Γ : List SExpr) → (σ : Subst) → (Δ : List SExpr) → Valuation → Prop
+  | nil : LR.Subst Γ .id Γ .nil
+  | cons : LR.Subst Γ σ.tail Δ ρ →
+    (∀ a, LE_Interp ρ a A →
+      (LR Γ).DefEq (A.subst σ.tail) (A.subst σ.tail) (.sort u) a .sort) →
+    LE_Interp ρ a A → (LR Γ).DefEq σ.head σ.head (A.subst σ.tail) x a →
+    LR.Subst Γ σ (A::Δ) (ρ.push x)
+
+theorem LR.Subst.fits (W : LR.Subst Γ σ Δ ρ) : ρ.Fits Γ Δ := sorry
+
+theorem LR.fundamental (H : Γ ⊢ M ≡ N : A) (W : LR.Subst Γ₀ σ Γ ρ)
+    (hM : LE_Interp ρ m M) :
+    ∃ a, LE_Interp ρ a A ∧ (LR Γ₀).DefEq (M.subst σ) (N.subst σ) (A.subst σ) m a := by
+  replace H := H.strong; induction H generalizing m with
+  | bvar h =>
+    sorry
+  | symm H ih =>
+    have hN := (LE_Interp.sound H.defeq W.fits).1.2 hM
+    have ⟨_, h1, h2⟩ := ih W hN; exact ⟨_, h1, h2.symm⟩
+  | trans _ H1 H2 ihA ih1 ih2 =>
+    have ⟨_, h1, h2⟩ := ih1 W hM
+    have hN := (LE_Interp.sound H1.defeq W.fits).1.1 hM
+    have ⟨_, h3, h4⟩ := ih2 W hN
+    have hJ := Shape.Join.mk (h1.compat h3)
+    have ⟨a1, a2⟩ := hJ.le; have a3 := h1.join hJ h3
+    have ⟨_, c1, c2⟩ := ihA W a3
+    exact have c2 := .mono_r_1 c1.le_sort .sort c2
+      ⟨_, a3, .trans (.mono_r_1 a1 c2 h2) (.mono_r_1 a2 c2 h4)⟩
+  | _ => sorry
